examples/dsls/mini_steel/Pulse.Soundness.Exists.fsti
@@ -81,3 +81,28 @@ val intro_exists_soundness
                  (mk_stt_ghost_comp uzero unit_tm emp_inames_tm
                     (pack_ln (Tv_App p (e, Q_Explicit)))
                     (mk_abs unit_tm Q_Explicit (mk_exists u a p))))
+
+(*
+
+ g |- a : Type u
+ g |- p : a -> vprop
+ g |- e : vprop
+ -------------------------------------------------------------------------
+ g |- intro_exists<u> #a p e : stt_ghost<0> unit empty (p e) (fun _ -> exists_ p)
+
+*)
+val intro_exists_erased_soundness
+  (#f:stt_env)
+  (#g:env)
+  (#u:universe)
+  (#a:term)
+  (#p:term)
+  (#e:term)
+  (a_typing:RT.typing (extend_env_l f g) a (pack_ln (Tv_Type u)))
+  (p_typing:RT.typing (extend_env_l f g) p (mk_arrow (a, Q_Explicit) vprop_tm))
+  (e_typing:RT.typing (extend_env_l f g) e (EPure.mk_erased u a))
+  : GTot (RT.typing (extend_env_l f g)
+                 (mk_intro_exists_erased u a p e)
+                 (mk_stt_ghost_comp uzero unit_tm emp_inames_tm
+                    (pack_ln (Tv_App p (EPure.mk_reveal u a e, Q_Explicit)))
+                    (mk_abs unit_tm Q_Explicit (mk_exists u a p))))
